theories/SetModel/CwF_library.v
@@ -1,0 +1,64 @@
+Require Import library.
+Require Import ZF_axioms.
+Require Import ZF_library.
+Require Import CwF.
+
+(* Defining terms and types using higher-order stuff *)
+
+Definition HO_Ty (n : nat) (Γ : ZFSet) (f : ZFSet -> ZFSet) := relToGraph Γ (𝕍 n × (ω × 𝕍 n)) (HO_rel f).
+Definition HO_Tm (n : nat) (Γ : ZFSet) (f : ZFSet -> ZFSet) := relToGraph Γ (𝕍 n) (HO_rel f).
+
+Lemma HO_Tm_pretyping {n : nat} {Γ : ZFSet} {f : ZFSet -> ZFSet} (Hf : ∀ γ ∈ Γ, f γ ∈ 𝕍 n) : HO_Tm n Γ f ∈ Γ ⇒ 𝕍 n.
+Proof.
+  apply relToGraph_typing. now apply HO_rel_typing.
+Qed.
+  
+Lemma cwfTy_to_depSet_HO_Ty {n : nat} {Γ γ : ZFSet} {f : ZFSet -> ZFSet} (Hf : ∀ γ ∈ Γ, f γ ∈ 𝕍 n × (ω × 𝕍 n)) (Hγ : γ ∈ Γ) :
+  cwfTy_to_depSet n Γ (HO_Ty n Γ f) γ ≡ setFstPair (𝕍 n) (ω × 𝕍 n) (f γ).
+Proof.
+  refine (fequal (setFstPair _ _) _).
+  now apply setAppArr_HO.
+Qed. 
+
+Lemma setAppArr_HO_Tm {n : nat} {Γ γ : ZFSet} {f : ZFSet -> ZFSet} (Hf : ∀ γ ∈ Γ, f γ ∈ 𝕍 n) (Hγ : γ ∈ Γ) : 
+  setAppArr Γ (𝕍 n) (HO_Tm n Γ f) γ ≡ f γ.
+Proof.
+  now apply setAppArr_HO.
+Qed.
+
+Lemma setAppArr_Tm_typing {n : nat} {Γ t : ZFSet} {A : ZFSet -> ZFSet}
+  (HA : ∀ γ ∈ Γ, A γ ∈ 𝕍 n × (ω × 𝕍 n)) (Ht : t ∈ Γ ⇒ 𝕍 n) :
+  (∀ γ ∈ Γ, setAppArr Γ (𝕍 n) t γ ∈ setFstPair (𝕍 n) (ω × 𝕍 n) (A γ)) -> (t ∈ cwfTm n Γ (HO_Ty n Γ A)).
+Proof.
+  intro Ht'. apply ZFincomp. split ; try assumption.
+  intros γ Hγ. refine (transpS (fun x => _ ∈ x) _ (Ht' γ Hγ)).
+  symmetry. now apply cwfTy_to_depSet_HO_Ty.
+Qed.
+
+Lemma setAppArr_Tm_detyping {n : nat} {Γ t : ZFSet} {A : ZFSet -> ZFSet}
+  (HA : ∀ γ ∈ Γ, A γ ∈ 𝕍 n × (ω × 𝕍 n)) :
+  (t ∈ cwfTm n Γ (HO_Ty n Γ A)) -> ∀ γ ∈ Γ, setAppArr Γ (𝕍 n) t γ ∈ setFstPair (𝕍 n) (ω × 𝕍 n) (A γ).
+Proof.
+  intros Ht' γ Hγ. apply ZFincomp in Ht'. destruct Ht' as [ _ Ht' ].
+  refine (transpS (fun x => _ ∈ x) _ (Ht' γ Hγ)).
+  now apply cwfTy_to_depSet_HO_Ty.
+Qed.
+
+Lemma HO_Tm_typing {n : nat} {Γ : ZFSet} {f A : ZFSet -> ZFSet}
+  (HA : ∀ γ ∈ Γ, A γ ∈ 𝕍 n × (ω × 𝕍 n)) :
+  (∀ γ ∈ Γ, f γ ∈ setFstPair (𝕍 n) (ω × 𝕍 n) (A γ)) -> (HO_Tm n Γ f ∈ cwfTm n Γ (HO_Ty n Γ A)).
+Proof.
+  intro H. assert (∀ γ ∈ Γ, f γ ∈ 𝕍 n) as Hf.
+  { intros γ Hγ. eapply ZFuniv_trans. now apply H. apply setFstPair_typing. now apply HA. }
+  eapply (setAppArr_Tm_typing HA (HO_Tm_pretyping Hf)).
+  intros γ Hγ. refine (transpS (fun x => x ∈ _) _ (H γ Hγ)).
+  symmetry. now apply setAppArr_HO_Tm.
+Qed.
+
+Lemma HO_Tm_detyping {n : nat} {Γ : ZFSet} {f A : ZFSet -> ZFSet}
+  (HA : ∀ γ ∈ Γ, A γ ∈ 𝕍 n × (ω × 𝕍 n)) (Hf : ∀ γ ∈ Γ, f γ ∈ 𝕍 n) :
+  (HO_Tm n Γ f ∈ cwfTm n Γ (HO_Ty n Γ A)) -> (∀ γ ∈ Γ, f γ ∈ setFstPair (𝕍 n) (ω × 𝕍 n) (A γ)).
+Proof.
+  intros H γ Hγ. eapply (setAppArr_Tm_detyping HA) in H.
+  refine (transpS (fun x => x ∈ _) _ H). now apply setAppArr_HO_Tm. assumption.
+Qed.
